feat: Std.Data.RBMap: part 3 (proof of erase)

Std/Data/RBMap.lean
@@ -308,40 +308,64 @@ protected theorem Ordered.insert (h : t.Ordered cmp) : (insert cmp t v).Ordered 
 /--
 The red-red invariant is a weakening of the red-black balance invariant which allows
 the root to be red with red children, but does not allow any other violations.
+It occurs as a temporary condition in the `insert` and `erase` functions.
+
+The `p` parameter allows the `.redred` case to be dependent on an additional condition.
+If it is false, then this is equivalent to the usual red-black invariant.
 -/
-inductive RedRed : RBNode α → Nat → Prop where
+inductive RedRed (p : Prop) : RBNode α → Nat → Prop where
   /-- A balanced tree has the red-red invariant. -/
-  | balanced : Balanced t c n → RedRed t n
-  /-- A red node with balanced red children has the red-red invariant. -/
-  | redred : Balanced a c₁ n → Balanced b c₂ n → RedRed (node red a x b) n
+  | balanced : Balanced t c n → RedRed p t n
+  /-- A red node with balanced red children has the red-red invariant (if `p` is true). -/
+  | redred : p → Balanced a c₁ n → Balanced b c₂ n → RedRed p (node red a x b) n
+
+/-- When `p` is false, the red-red case is impossible so the tree is balanced. -/
+protected theorem RedRed.of_false (h : ¬p) : RedRed p t n → ∃ c, Balanced t c n
+  | .balanced h => ⟨_, h⟩
+  | .redred hp .. => nomatch h hp
+
+/-- A `red` node with the red-red invariant has balanced children. -/
+protected theorem RedRed.of_red : RedRed p (node red a x b) n →
+    ∃ c₁ c₂, Balanced a c₁ n ∧ Balanced b c₂ n
+  | .balanced (.red ha hb) | .redred _ ha hb => ⟨_, _, ha, hb⟩
+
+/-- The red-red invariant is monotonic in `p`. -/
+protected theorem RedRed.imp (h : p → q) : RedRed p t n → RedRed q t n
+  | .balanced h => .balanced h
+  | .redred hp ha hb => .redred (h hp) ha hb
+
+/-- If `t` has the red-red invariant, then setting the root to black yields a balanced tree. -/
+protected theorem RedRed.setBlack : t.RedRed p n → ∃ n', (setBlack t).Balanced black n'
+  | .balanced h => h.setBlack
+  | .redred _ hl hr => ⟨_, hl.black hr⟩
 
 /-- The `balance1` function repairs the balance invariant when the first argument is red-red. -/
 protected theorem RedRed.balance1 {l : RBNode α} {v : α} {r : RBNode α}
-    (hl : l.RedRed n) (hr : r.Balanced c n) : ∃ c, (balance1 l v r).Balanced c (n + 1) := by
+    (hl : l.RedRed p n) (hr : r.Balanced c n) : ∃ c, (balance1 l v r).Balanced c (n + 1) := by
   unfold balance1; split
   case _ a x b y c => match hl with
-    | .redred (.red ha hb) hc => exact ⟨_, .red (.black ha hb) (.black hc hr)⟩
+    | .redred _ (.red ha hb) hc => exact ⟨_, .red (.black ha hb) (.black hc hr)⟩
   case _ a x b y c _ => match hl with
-    | .redred ha (.red hb hc) => exact ⟨_, .red (.black ha hb) (.black hc hr)⟩
+    | .redred _ ha (.red hb hc) => exact ⟨_, .red (.black ha hb) (.black hc hr)⟩
   case _ H1 H2 => match hl with
     | .balanced hl => exact ⟨_, .black hl hr⟩
-    | .redred (c₁ := black) (c₂ := black) ha hb => exact ⟨_, .black (.red ha hb) hr⟩
-    | .redred (c₁ := red) (.red ..) _ => cases H1 _ _ _ _ _ rfl
-    | .redred (c₂ := red) _ (.red ..) => cases H2 _ _ _ _ _ rfl
+    | .redred _ (c₁ := black) (c₂ := black) ha hb => exact ⟨_, .black (.red ha hb) hr⟩
+    | .redred _ (c₁ := red) (.red ..) _ => cases H1 _ _ _ _ _ rfl
+    | .redred _ (c₂ := red) _ (.red ..) => cases H2 _ _ _ _ _ rfl
 
-/-- The `balance2` function repairs the balance invariant when the first argument is red-red. -/
+/-- The `balance2` function repairs the balance invariant when the second argument is red-red. -/
 protected theorem RedRed.balance2 {l : RBNode α} {v : α} {r : RBNode α}
-    (hl : l.Balanced c n) (hr : r.RedRed n) : ∃ c, (balance2 l v r).Balanced c (n + 1) := by
+    (hl : l.Balanced c n) (hr : r.RedRed p n) : ∃ c, (balance2 l v r).Balanced c (n + 1) := by
   unfold balance2; split
   case _ a x b y c => match hr with
-    | .redred (.red ha hb) hc => exact ⟨_, .red (.black hl ha) (.black hb hc)⟩
+    | .redred _ (.red ha hb) hc => exact ⟨_, .red (.black hl ha) (.black hb hc)⟩
   case _ a x b y c _ => match hr with
-    | .redred ha (.red hb hc) => exact ⟨_, .red (.black hl ha) (.black hb hc)⟩
+    | .redred _ ha (.red hb hc) => exact ⟨_, .red (.black hl ha) (.black hb hc)⟩
   case _ H1 H2 => match hr with
     | .balanced hr => exact ⟨_, .black hl hr⟩
-    | .redred (c₁ := black) (c₂ := black) ha hb => exact ⟨_, .black hl (.red ha hb)⟩
-    | .redred (c₁ := red) (.red ..) _ => cases H1 _ _ _ _ _ rfl
-    | .redred (c₂ := red) _ (.red ..) => cases H2 _ _ _ _ _ rfl
+    | .redred _ (c₁ := black) (c₂ := black) ha hb => exact ⟨_, .black hl (.red ha hb)⟩
+    | .redred _ (c₁ := red) (.red ..) _ => cases H1 _ _ _ _ _ rfl
+    | .redred _ (c₂ := red) _ (.red ..) => cases H2 _ _ _ _ _ rfl
 
 /--
 The balance invariant of the `ins` function.
@@ -364,10 +388,10 @@ inductive InsBalanced : RBNode α → RBNode α → Nat → Prop where
   | redR : Balanced a black n → Balanced b black n → Balanced c black n →
     InsBalanced (node red a₀ v₀ b₀) (node red a x (node red b y c)) n
 
-protected theorem InsBalanced.redred {t₀ t : RBNode α} : t₀.InsBalanced t n → t.RedRed n
+protected theorem InsBalanced.redred {t₀ t : RBNode α} : t₀.InsBalanced t n → t.RedRed True n
   | .balanced h => .balanced h
-  | .redL ha hb hc => .redred (.red ha hb) hc
-  | .redR ha hb hc => .redred ha (.red hb hc)
+  | .redL ha hb hc => .redred ⟨⟩ (.red ha hb) hc
+  | .redR ha hb hc => .redred ⟨⟩ ha (.red hb hc)
 
 /-- The `ins` function is `ins`-balanced if the input is balanced. -/
 protected theorem Balanced.ins (cmp v) {t : RBNode α}
@@ -437,6 +461,10 @@ def setRed : RBNode α → RBNode α
   | node _ a v b => node red a v b
   | nil          => nil
 
+protected theorem All.setRed {t : RBNode α} (h : t.All p) : (setRed t).All p := by
+  unfold setRed; split <;> simp_all
+
+/-- The `setRed` function preserves the ordering invariants. -/
 protected theorem Ordered.setRed {t : RBNode α} : (setRed t).Ordered cmp ↔ t.Ordered cmp := by
   unfold setRed; split <;> simp [Ordered]
 
@@ -449,6 +477,47 @@ def balLeft (l : RBNode α) (v : α) (r : RBNode α) : RBNode α :=
     | node red (node black a y b) z c => node red (node black l v a) y (balance2 b z (setRed c))
     | r                               => node red l v r -- unreachable
 
+protected theorem All.balLeft
+    (hl : l.All p) (hv : p v) (hr : r.All p) : (balLeft l v r).All p := by
+  unfold balLeft; split <;> simp_all; split <;> simp_all [All.setRed]
+
+/-- The `balLeft` function preserves the ordering invariants. -/
+protected theorem Ordered.balLeft {l : RBNode α} {v : α} {r : RBNode α}
+    (lv : l.All (cmpLt cmp · v)) (vr : r.All (cmpLt cmp v ·))
+    (hl : l.Ordered cmp) (hr : r.Ordered cmp) : (balLeft l v r).Ordered cmp := by
+  unfold balLeft; split
+  · exact ⟨lv, vr, hl, hr⟩
+  split
+  · exact hl.balance2 lv vr hr
+  · have ⟨vy, va, _⟩ := vr.2.1; have ⟨⟨yz, _, bz⟩, zc, ⟨ay, yb, ha, hb⟩, hc⟩ := hr
+    exact ⟨⟨vy, vy.trans_r lv, ay⟩, balance2_All.2 ⟨yz, yb, (yz.trans_l zc).setRed⟩,
+      ⟨lv, va, hl, ha⟩, hb.balance2 bz zc.setRed (Ordered.setRed.2 hc)⟩
+  · exact ⟨lv, vr, hl, hr⟩
+
+/-- The balancing properties of the `balLeft` function. -/
+protected theorem Balanced.balLeft (hl : l.RedRed True n) (hr : r.Balanced cr (n + 1)) :
+    (balLeft l v r).RedRed (cr = red) (n + 1) := by
+  unfold balLeft; split
+  case _ a x b => exact
+    let ⟨ca, cb, ha, hb⟩ := hl.of_red
+    match cr with
+    | red => .redred rfl (.black ha hb) hr
+    | black => .balanced (.red (.black ha hb) hr)
+  case _ H =>
+    exact match hr with
+    | .black ha hb =>
+      match hl with
+      | .balanced hl => let ⟨c, h⟩ := RedRed.balance2 hl (.redred trivial ha hb); .balanced h
+      | .redred .. => nomatch H _ _ _ rfl
+    | .red (.black ha hb) hc =>
+      match hl with
+      | .balanced hl =>
+        match hc with
+        | .black hc hd =>
+          let ⟨c, h⟩ := RedRed.balance2 hb (.redred trivial hc hd)
+          .redred rfl (.black hl ha) h
+      | .redred .. => nomatch H _ _ _ rfl
+
 /-- Rebalancing a tree which has shrunk on the right. -/
 def balRight (l : RBNode α) (v : α) (r : RBNode α) : RBNode α :=
   match r with
@@ -457,6 +526,47 @@ def balRight (l : RBNode α) (v : α) (r : RBNode α) : RBNode α :=
     | node black a x b                => balance1 (node red a x b) v r
     | node red a x (node black b y c) => node red (balance1 (setRed a) x b) y (node black c v r)
     | l                               => node red l v r -- unreachable
+
+protected theorem All.balRight
+    (hl : l.All p) (hv : p v) (hr : r.All p) : (balRight l v r).All p := by
+  unfold balRight; split <;> simp_all; split <;> simp_all [All.setRed]
+
+/-- The `balRight` function preserves the ordering invariants. -/
+protected theorem Ordered.balRight {l : RBNode α} {v : α} {r : RBNode α}
+    (lv : l.All (cmpLt cmp · v)) (vr : r.All (cmpLt cmp v ·))
+    (hl : l.Ordered cmp) (hr : r.Ordered cmp) : (balRight l v r).Ordered cmp := by
+  unfold balRight; split
+  · exact ⟨lv, vr, hl, hr⟩
+  split
+  · exact hl.balance1 lv vr hr
+  · have ⟨yv, _, cv⟩ := lv.2.2; have ⟨ax, ⟨xy, xb, _⟩, ha, by_, yc, hb, hc⟩ := hl
+    exact ⟨balance1_All.2 ⟨xy, (xy.trans_r ax).setRed, by_⟩, ⟨yv, yc, yv.trans_l vr⟩,
+      (Ordered.setRed.2 ha).balance1 ax.setRed xb hb, cv, vr, hc, hr⟩
+  · exact ⟨lv, vr, hl, hr⟩
+
+/-- The balancing properties of the `balRight` function. -/
+protected theorem Balanced.balRight (hl : l.Balanced cl (n + 1)) (hr : r.RedRed True n) :
+    (balRight l v r).RedRed (cl = red) (n + 1) := by
+  unfold balRight; split
+  case _ b y c => exact
+    let ⟨cb, cc, hb, hc⟩ := hr.of_red
+    match cl with
+    | red => .redred rfl hl (.black hb hc)
+    | black => .balanced (.red hl (.black hb hc))
+  case _ H =>
+    exact match hl with
+    | .black hb hc =>
+      match hr with
+      | .balanced hr => let ⟨c, h⟩ := RedRed.balance1 (.redred trivial hb hc) hr; .balanced h
+      | .redred .. => nomatch H _ _ _ rfl
+    | .red hb (.black hc hd) =>
+      match hr with
+      | .balanced hr =>
+        match hb with
+        | .black ha hb =>
+          let ⟨c, h⟩ := RedRed.balance1 (.redred trivial ha hb) hc
+          .redred rfl h (.black hd hr)
+      | .redred .. => nomatch H _ _ _ rfl
 
 /-- The number of nodes in the tree. -/
 @[simp] def size : RBNode α → Nat
@@ -467,23 +577,11 @@ def balRight (l : RBNode α) (v : α) (r : RBNode α) : RBNode α :=
 The invariant of the `append` function. The main theorem is `Balanced.append`:
 if `l.Balanced c₁ n` and `r.Balanced c₂ n` then `(l.append r).AppendProp c₁ c₂ n`.
 -/
-inductive AppendProp : RBColor → RBColor → RBNode α → Nat → Prop
-  /-- It is always okay to make a balanced tree of black-height `n`. -/
-  | balanced : Balanced t c n → AppendProp c₁ c₂ t n
-  /-- It is okay to make a red-red tree of black-height `n`
-  as long as `c₁` and `c₂` are not both black. -/
-  | redder : (c₁ = black → c₂ ≠ black) →
-    Balanced x cx n → Balanced y cy n → AppendProp c₁ c₂ (node red x v y) n
-
-/-- The result of the append function is a red-red tree. -/
-theorem AppendProp.redred : AppendProp c₁ c₂ t n → t.RedRed n
-  | .balanced h => .balanced h
-  | .redder _ ha hb => .redred ha hb
+def AppendProp (c₁ c₂ : RBColor) (t : RBNode α) := t.RedRed (c₁ = black → c₂ ≠ black)
 
 /-- The result of the append function is a red-black tree when both inputs are black. -/
-theorem AppendProp.of_black : AppendProp black black t n → ∃ c, Balanced t c n
-  | .balanced h => ⟨_, h⟩
-  | .redder h _ _ => nomatch h rfl rfl
+theorem AppendProp.of_black (h : AppendProp black black t n) : ∃ c, Balanced t c n :=
+  h.of_false (· rfl rfl)
 
 /-- Concatenate two trees with the same black-height. -/
 def append : RBNode α → RBNode α → RBNode α
@@ -500,26 +598,71 @@ def append : RBNode α → RBNode α → RBNode α
   | node red a x b, c@(node black ..) => node red a x (append b c)
 termination_by _ x y => x.size + y.size
 
+protected theorem All.append (hl : l.All p) (hr : r.All p) : (append l r).All p := by
+  unfold append; split <;> simp [*]
+  · have ⟨hx, ha, hb⟩ := hl; have ⟨hy, hc, hd⟩ := hr
+    have := hb.append hc; split <;> simp_all
+  · have ⟨hx, ha, hb⟩ := hl; have ⟨hy, hc, hd⟩ := hr
+    have := hb.append hc; split <;> simp_all [All.balLeft]
+  · simp_all [hl.append hr.2.1]
+  · simp_all [hl.2.2.append hr]
+termination_by _ => l.size + r.size
+
+/-- The `append` function preserves the ordering invariants. -/
+protected theorem Ordered.append {l : RBNode α} {v : α} {r : RBNode α}
+    (lv : l.All (cmpLt cmp · v)) (vr : r.All (cmpLt cmp v ·))
+    (hl : l.Ordered cmp) (hr : r.Ordered cmp) : (append l r).Ordered cmp := by
+  unfold append; split
+  · exact hr
+  · exact hl
+  · have ⟨xv, _, bv⟩ := lv; have ⟨ax, xb, ha, hb⟩ := hl
+    have ⟨vy, vc, _⟩ := vr; have ⟨cy, yd, hc, hd⟩ := hr
+    have : _ ∧ _ ∧ _ := ⟨hb.append bv vc hc, xb.append (xv.trans_l vc), (vy.trans_r bv).append cy⟩
+    split
+    case _ H =>
+      have ⟨⟨b'z, c'z, hb', hc'⟩, ⟨xz, xb', _⟩, zy, _, c'y⟩ := H ▸ this
+      have az := xz.trans_r ax; have zd := zy.trans_l yd
+      exact ⟨⟨xz, az, b'z⟩, ⟨zy, c'z, zd⟩, ⟨ax, xb', ha, hb'⟩, c'y, yd, hc', hd⟩
+    · have ⟨hbc, xbc, bcy⟩ := this; have xy := xv.trans vy
+      exact ⟨ax, ⟨xy, xbc, xy.trans_l yd⟩, ha, bcy, yd, hbc, hd⟩
+  · have ⟨xv, _, bv⟩ := lv; have ⟨ax, xb, ha, hb⟩ := hl
+    have ⟨vy, vc, _⟩ := vr; have ⟨cy, yd, hc, hd⟩ := hr
+    have : _ ∧ _ ∧ _ := ⟨hb.append bv vc hc, xb.append (xv.trans_l vc), (vy.trans_r bv).append cy⟩
+    split
+    case _ H =>
+      have ⟨⟨b'z, c'z, hb', hc'⟩, ⟨xz, xb', _⟩, zy, _, c'y⟩ := H ▸ this
+      have az := xz.trans_r ax; have zd := zy.trans_l yd
+      exact ⟨⟨xz, az, b'z⟩, ⟨zy, c'z, zd⟩, ⟨ax, xb', ha, hb'⟩, c'y, yd, hc', hd⟩
+    · have ⟨hbc, xbc, bcy⟩ := this; have xy := xv.trans vy
+      exact ha.balLeft ax ⟨xy, xbc, xy.trans_l yd⟩ ⟨bcy, yd, hbc, hd⟩
+  · have ⟨vx, vb, _⟩ := vr; have ⟨bx, yc, hb, hc⟩ := hr
+    exact ⟨(vx.trans_r lv).append bx, yc, hl.append lv vb hb, hc⟩
+  · have ⟨xv, _, bv⟩ := lv; have ⟨ax, xb, ha, hb⟩ := hl
+    refine' ⟨ax, xb.append (xv.trans_l vr), ha, hb.append bv vr hr⟩
+termination_by _ l _ r _ _ _ _ => l.size + r.size
+
+/-- The balance properties of the `append` function. -/
 protected theorem Balanced.append {l r : RBNode α}
-    (hl : l.Balanced c₁ n) (hr : r.Balanced c₂ n) : (l.append r).AppendProp c₁ c₂ n := by
+    (hl : l.Balanced c₁ n) (hr : r.Balanced c₂ n) :
+    (l.append r).RedRed (c₁ = black → c₂ ≠ black) n := by
   unfold append; split
   case _ x => exact .balanced hr
   case _ x _ => exact .balanced hl
   case _ a x b c y d =>
     have .red ha hb := hl; have .red hc hd := hr
-    have ⟨_, IH⟩ := (hb.append hc).of_black; split
+    have ⟨_, IH⟩ := (hb.append hc).of_false (· rfl rfl); split
     case _ b' z c' e =>
       have .red hb' hc' := e ▸ IH
-      exact .redder (fun.) (.red ha hb') (.red hc' hd)
+      exact .redred (fun.) (.red ha hb') (.red hc' hd)
     case _ bcc _ H =>
       match bcc, append b c, IH, H with
-      | black, _, IH, _ => refine' .redder (fun.) ha (.red IH hd)
+      | black, _, IH, _ => refine' .redred (fun.) ha (.red IH hd)
       | red, _, .red .., H => cases H _ _ _ rfl
   case _ a x b c y d =>
     have .black ha hb := hl; have .black hc hd := hr
     have IH := hb.append hc; split
     case _ b' z c' e => match e ▸ IH with
-      | .balanced (.red hb' hc') | .redder _ hb' hc' =>
+      | .balanced (.red hb' hc') | .redred _ hb' hc' =>
         exact .balanced (.red (.black ha hb') (.black hc' hd))
     case _ cc dc _ H =>
       match append b c, IH, H with
@@ -529,28 +672,36 @@ protected theorem Balanced.append {l r : RBNode α}
           have .red ha' hb' := ha
           exact .balanced (.red (.black ha' hb') (.black hbc hd))
         case _ _ x b =>
-          exact have ⟨c, h⟩ := RedRed.balance2 ha (.redred hbc hd); .balanced h
-      | _, .redder .., H => cases H _ _ _ rfl
+          exact have ⟨c, h⟩ := RedRed.balance2 ha (.redred trivial hbc hd); .balanced h
+      | _, .redred .., H => cases H _ _ _ rfl
   case _ a x b c y d =>
     have .red hc hd := hr; have IH := hl.append hc
-    have .black ha hb := hl; have ⟨c, IH⟩ := IH.of_black
-    exact .redder (fun.) IH hd
+    have .black ha hb := hl; have ⟨c, IH⟩ := IH.of_false (· rfl rfl)
+    exact .redred (fun.) IH hd
   case _ a x b c y d =>
     have .red ha hb := hl; have IH := hb.append hr
-    have .black hc hd := hr; have ⟨c, IH⟩ := IH.of_black
-    exact .redder (fun.) ha IH
+    have .black hc hd := hr; have ⟨c, IH⟩ := IH.of_false (· rfl rfl)
+    exact .redred (fun.) ha IH
 termination_by _ x y _ _ => x.size + y.size
 
 /-! ## erase -/
 
-/-- The invariant of the `del` function. -/
-inductive DelProp : RBNode α → RBNode α → Nat → Prop
-  /-- If the input tree is red or nil, then the result of deletion is a balanced tree with
-  some color and the same black-height. -/
-  | balanced : t₀.isBlack = false → Balanced t c n → DelProp t₀ t n
-  /-- If the input tree is black, then the result of deletion is a red-red tree with
-  black-height lowered by 1. -/
-  | redred : t₀.isBlack = true → RedRed t n → DelProp t₀ t (n + 1)
+/--
+The invariant of the `del` function.
+* If the input tree is black, then the result of deletion is a red-red tree with
+  black-height lowered by 1.
+* If the input tree is red or nil, then the result of deletion is a balanced tree with
+  some color and the same black-height.
+-/
+def DelProp (t₀ t : RBNode α) (n : Nat) : Prop :=
+  bif t₀.isBlack then ∃ n', n = n' + 1 ∧ RedRed True t n' else ∃ c, Balanced t c n
+
+/-- The `DelProp` property is a strengthened version of the red-red invariant. -/
+theorem DelProp.redred (h : DelProp t₀ t n) : ∃ n', RedRed t₀.isBlack t n' := by
+  unfold DelProp at h
+  exact match t₀.isBlack, h with
+  | false, ⟨_, h⟩ => ⟨_, .balanced h⟩
+  | true, ⟨_, _, h⟩ => ⟨_, h.imp fun _ => rfl⟩
 
 /--
 The core of the `erase` function. The tree returned from this function has a broken invariant,
@@ -564,6 +715,57 @@ which is restored in `erase`.
     | .gt => bif b.isBlack then balRight a y (del cut b) else node red a y (del cut b)
     | .eq => append a b
 
+protected theorem All.del : ∀ {t : RBNode α}, t.All p → (del cut t).All p
+  | .nil, h => h
+  | .node .., ⟨hy, ha, hb⟩ => by
+    unfold del; split
+    · unfold cond; split
+      · exact ha.del.balLeft hy hb
+      · exact ⟨hy, ha.del, hb⟩
+    · unfold cond; split
+      · exact ha.balRight hy hb.del
+      · exact ⟨hy, ha, hb.del⟩
+    · exact ha.append hb
+
+/-- The `del` function preserves the ordering invariants. -/
+protected theorem Ordered.del : ∀ {t : RBNode α}, t.Ordered cmp → (del cut t).Ordered cmp
+  | .nil, _ => ⟨⟩
+  | .node _ a y b, ⟨ay, yb, ha, hb⟩ => by
+    unfold del; split
+    · unfold cond; split
+      · exact ha.del.balLeft ay.del yb hb
+      · exact ⟨ay.del, yb, ha.del, hb⟩
+    · unfold cond; split
+      · exact ha.balRight ay yb.del hb.del
+      · exact ⟨ay, yb.del, ha, hb.del⟩
+    · exact ha.append ay yb hb
+
+/-- The `del` function has the `DelProp` property. -/
+protected theorem Balanced.del {t : RBNode α} (h : t.Balanced c n) : t.DelProp (t.del cut) n := by
+  induction h with
+  | nil => exact ⟨_, .nil⟩
+  | @black a ca n b cb v ha hb iha ihb =>
+    refine ⟨_, rfl, ?_⟩
+    unfold del; split
+    · exact match a, n, iha with
+      | .nil, _, ⟨c, ha⟩
+      | .node red .., _, ⟨c, ha⟩ => .redred ⟨⟩ ha hb
+      | .node black .., _, ⟨n, rfl, ha⟩ => (hb.balLeft ha).imp fun _ => ⟨⟩
+    · exact match b, n, ihb with
+      | .nil, _, ⟨c, hb⟩
+      | .node .red .., _, ⟨c, hb⟩ => .redred ⟨⟩ ha hb
+      | .node black .., _, ⟨n, rfl, hb⟩ => (ha.balRight hb).imp fun _ => ⟨⟩
+    · exact (ha.append hb).imp fun _ => ⟨⟩
+  | @red a n b v ha hb iha ihb =>
+    unfold del; split
+    · exact match a, n, iha with
+      | .nil, _, _ => ⟨_, .red ha hb⟩
+      | .node black .., _, ⟨n, rfl, ha⟩ => (hb.balLeft ha).of_false (fun.)
+    · exact match b, n, ihb with
+      | .nil, _, _ => let .nil := hb; ⟨_, .red ha .nil⟩
+      | .node black .., _, ⟨n, rfl, hb⟩ => (ha.balRight hb).of_false (fun.)
+    · exact (ha.append hb).of_false (· rfl rfl)
+
 /--
 The `erase cut t` function removes an element from the tree `t`.
 The `cut` function is used to locate an element in the tree:
@@ -573,6 +775,15 @@ if it returns `.eq` we will remove the element.
 are not of this form as long as they are suitably monotonic.)
 -/
 @[specialize] def erase (cut : α → Ordering) (t : RBNode α) : RBNode α := (del cut t).setBlack
+
+/-- The `erase` function preserves the ordering invariants. -/
+protected theorem Ordered.erase {t : RBNode α} (h : t.Ordered cmp) : (erase cut t).Ordered cmp :=
+  Ordered.setBlack.2 h.del
+
+/-- The `erase` function preserves the balance invariants. -/
+protected theorem Balanced.erase {t : RBNode α}
+    (h : t.Balanced c n) : ∃ n, (t.erase cut).Balanced black n :=
+  have ⟨_, h⟩ := (h.del (cut := cut)).redred; h.setBlack
 
 section Membership
 
@@ -672,9 +883,16 @@ instance [Repr α] : Repr (RBTree α cmp) where
 @[inline] def insert (t : RBTree α cmp) (v : α) : RBTree α cmp :=
   ⟨t.1.insert cmp v, let ⟨o, _, _, h⟩ := t.2; ⟨o.insert, h.insert⟩⟩
 
--- TODO
--- @[inline] def erase : RBTree α cmp → α → RBTree α cmp
---   | ⟨t, w⟩, k => ⟨t.erase cmp k, WellFormed.eraseWff w rfl⟩
+/--
+`O(log n)`. Remove an element from the tree using a cut function.
+The `cut` function is used to locate an element in the tree:
+it returns `.gt` if we go too high and `.lt` if we go too low;
+if it returns `.eq` we will remove the element.
+(The function `cmp k` for some key `k` is a valid cut function, but we can also use cuts that
+are not of this form as long as they are suitably monotonic.)
+-/
+@[inline] def erase (t : RBTree α cmp) (cut : α → Ordering) : RBTree α cmp :=
+  ⟨t.1.erase cut, let ⟨o, _, _, h⟩ := t.2; ⟨o.erase, _, h.erase⟩⟩
 
 /-- `O(log n)`. Find an element in the tree using a cut function. -/
 @[inline] def findP? (t : RBTree α cmp) (cut : α → Ordering) : Option α := t.1.find? cut
@@ -826,9 +1044,8 @@ instance [Repr α] [Repr β] : Repr (RBMap α β cmp) where
 /-- `O(log n)`. Insert key-value pair `(k,v)` into the tree. -/
 @[inline] def insert (t : RBMap α β cmp) (k : α) (v : β) : RBMap α β cmp := RBTree.insert t (k, v)
 
--- TODO
--- @[inline] def erase : RBMap α β cmp → α → RBMap α β cmp
---   | ⟨t, w⟩, k => ⟨t.erase cmp k, WellFormed.eraseWff w rfl⟩
+/-- `O(log n)`. Remove an element `k` from the map. -/
+@[inline] def erase (t : RBMap α β cmp) (k : α) : RBMap α β cmp := RBTree.erase t (cmp k ·.1)
 
 /-- `O(n log n)`. Build a tree from an unsorted list by inserting them one at a time. -/
 @[inline] def ofList (l : List (α × β)) (cmp : α → α → Ordering) : RBMap α β cmp :=
